incomplete edits

intermediate/Veritas.Intermediate.Logs.fst
@@ -1,6 +1,6 @@
-
 module Veritas.Intermediate.Logs
 
+open Veritas.Interleave
 open Veritas.Key
 open Veritas.MultiSetHashDomain
 open Veritas.Record
@@ -43,7 +43,26 @@ let to_state_op (e:logS_entry {is_state_op e}): Veritas.State.state_op =
 let to_state_op_logS (l: logS) =
   map to_state_op (filter_refine is_state_op l)
 
+(* Reproducing definitions from Veritas.Verifier.Thread *)
+
 let thread_id_logS = thread_id & logS
+
+let thread_id_of (tl: thread_id_logS): nat = fst tl
+
+let logS_of (tl: thread_id_logS): logS = snd tl
+
+let tl_length (tl: thread_id_logS): nat =
+  Seq.length (logS_of tl)
+
+let tl_idx (tl: thread_id_logS) = i:nat{i < tl_length tl}
+
+let tl_index (tl: thread_id_logS) (i:tl_idx tl): logS_entry =
+  Seq.index (logS_of tl) i
+
+let tl_prefix (tl: thread_id_logS) (i:nat{i <= tl_length tl}): thread_id_logS =
+  (thread_id_of tl), (prefix (logS_of tl) i)
+
+(* Reproducing definitions from Veritas.Verifier.Global *)
 
 let g_logS = Seq.seq logS
 
@@ -52,3 +71,13 @@ let thread_log (gl: g_logS) (tid: seq_index gl): thread_id_logS =
 
 let to_state_op_glogS (gl: g_logS) =
   map to_state_op_logS gl
+
+(* Reproducing definitions from Veritas.Verifier.TSLog *)
+
+let il_logS = interleaving logS_entry
+
+let thread_count (il:il_logS) = Seq.length (s_seq il)
+
+let valid_tid (il:il_logS) = tid:nat{tid < thread_count il}
+
+let g_logS_of (il: il_logS): g_logS = s_seq il
